added a test that shows how jar2bpl creates a wrong encoding of the partial order.

gravy/test/out.bpl
@@ -2,132 +2,60 @@ type ref;
 type javaType;
 type Field $GenericType__0;
 type $heap_type = <$GenericType__0>[ref,Field $GenericType__0]$GenericType__0;
-type boolArrHeap_type = [ref][int]bool;
-type refArrHeap_type = [ref][int]ref;
-type realArrHeap_type = [ref][int]int;
-type intArrHeap_type = [ref][int]int;
-const unique $null : ref;
+
 const unique $type : Field javaType;
 const unique $alloc : Field bool;
+const unique $null : ref;
 const { :sourceloc "Object.java",-1,-1,-1,-1 } unique java.lang.Object : javaType extends  complete;
-const { :sourceloc "FalsePositives.java",-1,-1,-1,-1 } unique FalsePositives : javaType extends  unique java.lang.Object complete;
-const { :sourceloc "Serializable.java",-1,-1,-1,-1 } unique java.io.Serializable : javaType extends  unique java.lang.Object complete;
-const { :sourceloc "Comparable.java",-1,-1,-1,-1 } unique java.lang.Comparable : javaType extends  unique java.lang.Object complete;
-const { :sourceloc "CharSequence.java",-1,-1,-1,-1 } unique java.lang.CharSequence : javaType extends  unique java.lang.Object complete;
-const { :sourceloc "String.java",-1,-1,-1,-1 } unique java.lang.String : javaType extends  unique java.lang.CharSequence, unique java.lang.Object, unique java.lang.Comparable, unique java.io.Serializable complete;
-const unique $StringConst0 : ref extends  complete;
-const unique $StringConst1 : ref extends  complete;
-const unique $StringConst2 : ref extends  complete;
+const { :sourceloc "FalsePositives03.java",-1,-1,-1,-1 } unique FalsePositives03 : javaType extends  unique java.lang.Object complete;
+const { :sourceloc "Context.java",-1,-1,-1,-1 } unique javax.naming.Context : javaType extends  unique java.lang.Object complete;
 var $heap : $heap_type;
-var $intArrayType : javaType;
-var $charArrayType : javaType;
-var $boolArrayType : javaType;
-var $byteArrayType : javaType;
-var $longArrayType : javaType;
-var $arrSizeHeap : [ref]int;
-var $stringSizeHeap : [ref]int;
-var $boolArrHeap : boolArrHeap_type;
-var $refArrHeap : refArrHeap_type;
-var $realArrHeap : realArrHeap_type;
-var $intArrHeap : intArrHeap_type;
-var int$FalsePositives$countSource0 : Field int;
-function $arrayType(t:javaType) returns ($ret:javaType);
+
+
 function $intToReal(x:int) returns ($ret:real);
 function $intToBool(x:int) returns ($ret:bool) { (if x == 0 then false else true) }
 function $refToBool(x:ref) returns ($ret:bool) { (if x == $null then false else true) }
 function $boolToInt(x:bool) returns ($ret:int) { (if x == true then 1 else 0) }
-function $cmpBool(x:bool, y:bool) returns ($ret:int);
-function $cmpRef(x:ref, y:ref) returns ($ret:int);
-function $cmpReal(x:real, y:real) returns ($ret:int) { (if x > y then 1 else (if x < y then -1 else 0)) }
-function $cmpInt(x:int, y:int) returns ($ret:int) { (if x > y then 1 else (if x < y then -1 else 0)) }
-function $bitOr(x:int, y:int) returns ($ret:int);
-function $bitAnd(x:int, y:int) returns ($ret:int);
-function $xorInt(x:int, y:int) returns ($ret:int);
-function $shlInt(x:int, y:int) returns ($ret:int);
-function $ushrInt(x:int, y:int) returns ($ret:int);
-function $shrInt(x:int, y:int) returns ($ret:int);
-procedure $new(obj_type:javaType) returns ($obj:ref);        requires $heap[$obj,$alloc] == false;    ensures $heap[$obj,$type] == obj_type;    ensures $heap[$obj,$alloc] == true;    ensures $obj != $null;
 
-procedure java.lang.Object$java.lang.Object$clone$43($this:ref) returns ($other:ref);    ensures $heap[$other,$type] == $heap[$this,$type];    ensures $heap[$other,$alloc] == true;        ensures $other != $null;
 
-procedure int$java.lang.String$compareTo$87($this:ref, $other:ref) returns ($return:int); 
 
-procedure void$FalsePositives$FalsePositive02$1889($this:ref, $in_parameter__0:ref) returns ($exception:ref);    modifies $heap;
 
-procedure java.lang.String$java.lang.Object$toString$44($this:ref) returns ($return:ref, $exception:ref);    
+procedure void$FalsePositives03$foo$1889($this:ref, $in_parameter__0:ref) returns ($exception:ref);    
 
-procedure void$FalsePositives$$la$init$ra$$1890($this:ref) returns ($exception:ref);    
 
-procedure void$java.lang.Object$$la$init$ra$$38($this:ref) returns ($exception:ref);    
-
-implementation void$FalsePositives$FalsePositive02$1889($this:ref, $in_parameter__0:ref) returns ($exception:ref){
+implementation void$FalsePositives03$foo$1889($this:ref, $in_parameter__0:ref) returns ($exception:ref){
     
-var temp$25 : int;    
-var temp$710 : int;    
-var htmlTag2 : ref;    
-var temp$36 : ref;    
-var temp$47 : int;    
-var temp$58 : int;    
-var temp$811 : int;    
-var temp$03 : ref;    
-var temp$69 : ref;    
+var temp$03 : int;    
+var ctx4 : ref;    
 var this1 : ref;    
-var temp$14 : int;
+var container2 : ref;
     assume $this != $null;
     this1 := $this;
-    htmlTag2 := $in_parameter__0;
-    assert { :sourceloc "FalsePositives.java",67,7,67,47 } htmlTag2 != $null;
-    call temp$03, $exception := java.lang.String$java.lang.Object$toString$44(htmlTag2);
-    assert { :sourceloc "FalsePositives.java",67,7,67,47 } temp$03 != $null;
-    call temp$14 := int$java.lang.String$compareTo$87(temp$03, $StringConst0);
-    if (temp$14 == 0) {
-        assert { :sourceloc "FalsePositives.java",67,7,67,47 } true;
+    container2 := $in_parameter__0;
+    temp$03 := $boolToInt($heap[container2,$type] <: javax.naming.Context);
+    if (temp$03 == 0) {
+        assert { :sourceloc "FalsePositives03.java",15,13,15,40 } true;
         goto block1;
     } else {
-        assert { :sourceloc "FalsePositives.java",67,7,67,47 } true;
+        assert { :sourceloc "FalsePositives03.java",15,13,15,40 } true;
     }
     goto block2;
   block1:
-    temp$25 := 1;
-    assert { :sourceloc "FalsePositives.java",69,4,69,14 } this1 != $null;
-    $heap := $heap[this1,int$FalsePositives$countSource0 := temp$25];
+    if (container2 == $null) {
+        assert { :sourceloc "FalsePositives03.java",15,45,15,61 } true;
+        goto block2;
+    } else {
+        assert { :sourceloc "FalsePositives03.java",15,45,15,61 } true;
+    }
+    goto block3;
     goto block3;
   block2:
-    assert { :sourceloc "FalsePositives.java",71,12,71,49 } htmlTag2 != $null;
-    call temp$36, $exception := java.lang.String$java.lang.Object$toString$44(htmlTag2);
-    assert { :sourceloc "FalsePositives.java",71,12,71,49 } temp$36 != $null;
-    call temp$47 := int$java.lang.String$compareTo$87(temp$36, $StringConst1);
-    if (temp$47 == 0) {
-        assert { :sourceloc "FalsePositives.java",71,12,71,49 } true;
-        goto block4;
-    } else {
-        assert { :sourceloc "FalsePositives.java",71,12,71,49 } true;
-    }
-    goto block5;
-  block4:
-    temp$58 := 2;
-    assert { :sourceloc "FalsePositives.java",73,4,73,14 } this1 != $null;
-    $heap := $heap[this1,int$FalsePositives$countSource0 := temp$58];
-    goto block6;
-  block5:
-    assert { :sourceloc "FalsePositives.java",75,12,75,49 } htmlTag2 != $null;
-    call temp$69, $exception := java.lang.String$java.lang.Object$toString$44(htmlTag2);
-    assert { :sourceloc "FalsePositives.java",75,12,75,49 } temp$69 != $null;
-    call temp$710 := int$java.lang.String$compareTo$87(temp$69, $StringConst2);
-    if (temp$710 == 0) {
-        assert { :sourceloc "FalsePositives.java",75,12,75,49 } true;
-        goto block7;
-    } else {
-        assert { :sourceloc "FalsePositives.java",75,12,75,49 } true;
-    }
-    goto block8;
-  block7:
-    temp$811 := 3;
-    assert { :sourceloc "FalsePositives.java",77,4,77,14 } this1 != $null;
-    $heap := $heap[this1,int$FalsePositives$countSource0 := temp$811];
-  block8:
-  block6:
+    assert { :sourceloc "FalsePositives03.java",16,13,16,48 } $heap[container2,$type] <: javax.naming.Context;
+    ctx4 := container2;
+    goto block4;
   block3:
+  block4:
     return;
 }
+
 
